All tests compile

Source/DafnyCore.Test/GeneratedDafnyTest.cs
@@ -18,4 +18,9 @@ public class GeneratedDafnyTest {
   public void TestPathSimplification() {
     FactorPathsOptimizationTest.__default.TestApply();
   }
+
+  [Fact]
+  public void TestDefsCoverage() {
+    DefsCoverage.__default.Test(); ;
+  }
 }
