Source/DafnyCore/Backends/Rust/Dafny-compiler-rust-definitions.dfy
@@ -179,6 +179,9 @@ module {:extern "Defs"} DafnyToRustCompilerDefinitions {
     predicate NeedsAsRefForBorrow(name: string) {
       name in types && types[name].NeedsAsRefForBorrow()
     }
+    predicate IsMaybePlacebo(name: string) {
+      name in types && types[name].ExtractMaybePlacebo().Some?
+    }
     function AddAssigned(name: string, tpe: R.Type): Environment
       // If we know for sure the type of name extends the Copy trait
     {
@@ -203,11 +206,14 @@ module {:extern "Defs"} DafnyToRustCompilerDefinitions {
         assignmentStatusKnown - {name}
       )
     }
-    function AddAssignmentStatusKnown(name: string): Environment {
+    function AddAssignmentStatus(name: string, assignmentStatus: AssignmentStatus): Environment {
       Environment(
         names,
         types,
-        assignmentStatusKnown + {name}
+        if assignmentStatus.Unknown? then
+          assignmentStatusKnown - {name}
+        else
+          assignmentStatusKnown + {name}
       )
     }
     predicate IsAssignmentStatusKnown(name: string) {
@@ -761,5 +767,80 @@ module {:extern "Defs"} DafnyToRustCompilerDefinitions {
       case Print(_) => DetectAssignmentStatus(stmts_remainder[1..], dafny_name)
       case _ => Unknown
     }
+  }
+}
+
+// Tests
+module {:extern "DefsCoverage"} DafnyToRustCompilerDefinitionsCoverage {
+  import opened DafnyToRustCompilerDefinitions
+  import opened DAST
+  import Strings = Std.Strings
+  import Std
+  import opened Std.Wrappers
+  import R = RAST
+  import opened DafnyCompilerRustUtils
+
+  const IND := R.IND
+  type Type = DAST.Type
+  type Formal = DAST.Formal
+
+  method Expect(x: bool)
+  {
+    expect x; // Avoids having too little coverage
+  }
+
+  method Tests() {
+    Expect(SurelyAssigned.Join(SurelyAssigned) == SurelyAssigned);
+    Expect(NotAssigned.Join(NotAssigned) == NotAssigned);
+    Expect(NotAssigned.Join(SurelyAssigned) == Unknown);
+    Expect(SurelyAssigned.Join(NotAssigned) == Unknown);
+    Expect(Unknown.Join(NotAssigned) == NotAssigned.Join(Unknown) == Unknown);
+    Expect(Unknown.Join(SurelyAssigned) == SurelyAssigned.Join(Unknown) == Unknown);
+    Expect(Unknown.Join(Unknown) == Unknown);
+    
+    Expect(SurelyAssigned.Then(Unknown)
+                   == SurelyAssigned.Then(NotAssigned)
+                   == SurelyAssigned.Then(SurelyAssigned)
+                   == NotAssigned.Then(SurelyAssigned)
+                   == SurelyAssigned);
+    Expect(Unknown.Then(NotAssigned)
+                   == Unknown.Then(SurelyAssigned)
+                   == Unknown.Then(Unknown)
+                   == NotAssigned.Then(Unknown)
+                   == Unknown);
+    Expect(NotAssigned.Then(NotAssigned)
+                   == NotAssigned);
+    
+    var x := VarName("x");
+    var y := VarName("y");
+    var z := Expression.Ident(VarName("z"));
+    var assigns_x := [Assign(AssignLhs.Ident(x), Expression.Ident(y))];
+    var assigns_y := [Assign(AssignLhs.Ident(y), Expression.Ident(x))];
+    var cond := Expression.Ident(VarName("cond"));
+    var unknown_x := [If(cond, assigns_x, assigns_y)];
+    var surely_double_x := [If(cond, assigns_x, assigns_x)];
+    var call_to_x := [Statement.Call(z, SetBuilderAdd, [], [], Some([x]))];
+    var declare_x_again := [DeclareVar(x, Type.Tuple([]), None)];
+    Expect(DetectAssignmentStatus(assigns_y, x) == NotAssigned);
+    Expect(DetectAssignmentStatus(assigns_x, x) == SurelyAssigned);
+    Expect(DetectAssignmentStatus(assigns_x, y) == NotAssigned);
+    Expect(DetectAssignmentStatus(assigns_x + assigns_y, y) == SurelyAssigned);
+    Expect(DetectAssignmentStatus(unknown_x, x) == Unknown);
+    Expect(DetectAssignmentStatus(surely_double_x, x) == SurelyAssigned);
+    Expect(DetectAssignmentStatus(surely_double_x, y) == NotAssigned);
+    Expect(DetectAssignmentStatus(call_to_x, x) == SurelyAssigned);
+    Expect(DetectAssignmentStatus(call_to_x, y) == NotAssigned);
+    Expect(DetectAssignmentStatus(call_to_x + assigns_y, y) == SurelyAssigned);
+    Expect(DetectAssignmentStatus([Labeled("l", assigns_y)] + assigns_x, y) == SurelyAssigned);
+    Expect(DetectAssignmentStatus([Labeled("l", assigns_x)] + assigns_y, x) == SurelyAssigned);
+    Expect(DetectAssignmentStatus([Labeled("l", assigns_x)] + assigns_y, x) == SurelyAssigned);
+    Expect(DetectAssignmentStatus(declare_x_again + assigns_x, x) == NotAssigned);
+    Expect(DetectAssignmentStatus(declare_x_again + assigns_y, y) == SurelyAssigned);
+    Expect(DetectAssignmentStatus([Return(z)] + assigns_x, x) == NotAssigned);
+    Expect(DetectAssignmentStatus([EarlyReturn()] + assigns_x, x) == NotAssigned);
+    Expect(DetectAssignmentStatus([JumpTailCallStart()] + assigns_x, x) == NotAssigned);
+    Expect(DetectAssignmentStatus([Print(z)] + assigns_x, x) == SurelyAssigned);
+    Expect(DetectAssignmentStatus([Print(z)] + assigns_x, x) == SurelyAssigned);
+    Expect(DetectAssignmentStatus([While(z, [])] + assigns_x, x) == Unknown);
   }
 }
